Proved the high-level correctness of insertion

examples/low-level/merkletree/MerkleTree.High.fst
@@ -3,12 +3,14 @@ module MerkleTree.High
 open FStar.All
 open FStar.Mul
 open FStar.Seq
+// open FStar.BitVector
 
 // open EverCrypt.Hash
 // open MerkleTree.Spec
 
 module List = FStar.List.Tot
 module S = FStar.Seq
+module BV = FStar.BitVector
 
 assume type elem: eqtype u#0
 assume type hash: eqtype u#0
@@ -22,7 +24,7 @@ assume val hash_from_hashes: hash -> hash -> Tot hash
 assume val hash_init_idem: 
   h:hash -> Lemma (hash_from_hashes h hash_init = h)
 
-/// Mapping sequences (why is it not in the library?)
+/// About FStar.Seq.Base.seq (the library is not that rich enough..)
 
 val seq_map:
   #a:Type -> #b:Type -> f:(a -> b) -> s:S.seq a -> 
@@ -33,6 +35,33 @@ val seq_map:
 let rec seq_map #a #b f s =
   if S.length s = 0 then S.empty
   else S.cons (f (S.head s)) (seq_map f (S.tail s))
+
+val seq_map_create:
+  #a:Type -> #b:Type -> f:(a -> b) -> 
+  len:nat -> ia:a ->
+  Lemma (seq_map f (S.create len ia) ==
+	S.create len (f ia))
+	[SMTPat (seq_map f (S.create len ia))]
+let rec seq_map_create #a #b f len ia =
+  S.lemma_eq_intro (seq_map f (S.create len ia)) (S.create len (f ia))
+  // S.lemma_eq_elim (seq_map f (S.create len ia)) (S.create len (f ia))
+
+val seq_map_append:
+  #a:Type -> #b:Type -> f:(a -> b) -> 
+  s1:S.seq a -> s2:S.seq a ->
+  Lemma (seq_map f (S.append s1 s2) ==
+	S.append (seq_map f s1) (seq_map f s2))
+	[SMTPat (seq_map f (S.append s1 s2))]
+let rec seq_map_append #a #b f s1 s2 =
+  S.lemma_eq_elim (seq_map f (S.append s1 s2)) 
+		  (S.append (seq_map f s1) (seq_map f s2))
+
+val lemma_split_append:
+  #a:Type -> s1:S.seq a -> s2:S.seq a ->
+  Lemma (S.split (S.append s1 s2) (S.length s1) == (s1, s2))
+let lemma_split_append #a s1 s2 =
+  S.lemma_eq_elim (fst (S.split (S.append s1 s2) (S.length s1))) s1;
+  S.lemma_eq_elim (snd (S.split (S.append s1 s2) (S.length s1))) s2
 
 /// Power of two (TODO: use a bit vector; division is expensive)
 
@@ -75,6 +104,7 @@ val pow2_floor_is_pow2:
   n:nat ->
   Lemma (requires (is_pow2 n))
 	(ensures (n = pow2 (pow2_floor n)))
+	[SMTPat (is_pow2 n)]
 let rec pow2_floor_is_pow2 n =
   if n = 1 then ()
   else pow2_floor_is_pow2 (n / 2)
@@ -94,27 +124,47 @@ let pow2_interval_unique n p1 p2 =
 val pow2_floor_inv:
   p:nat -> n:nat{pow2 p <= n && n < pow2 (p + 1)} ->
   Lemma (pow2_floor n = p)
-let rec pow2_floor_inv p n =
+let pow2_floor_inv p n =
   pow2_interval_unique n (pow2_floor n) p
+
+val pow2_floor_pow2_less:
+  p:nat -> n:nat{n < pow2 p} ->
+  Lemma (pow2_floor (pow2 p + n) = p)
+let pow2_floor_pow2_less p n =
+  pow2_floor_inv p (pow2 p + n)
 
 val pow2_floor_pow2_pow2:
   p:nat -> q:nat{p > q} ->
   Lemma (pow2_floor (pow2 p + pow2 q) = p)
-let rec pow2_floor_pow2_pow2 p q =
+let pow2_floor_pow2_pow2 p q =
   Math.Lemmas.pow2_lt_compat p q;
-  pow2_floor_inv p (pow2 p + pow2 q)
+  pow2_floor_pow2_less p (pow2 q)
 
 /// Invariants between internal roots and values
 
+type hash_seq_pow2 = hs:hash_seq{is_pow2 (S.length hs)}
+type elem_seq_pow2 = vs:elem_seq{is_pow2 (S.length vs)}
+
 val merkle_root_of_pow2:
-  #nelts:nat{is_pow2 nelts} -> vs:hash_seq{S.length vs = nelts} -> 
-  GTot hash
-let rec merkle_root_of_pow2 #nelts vs =
-  if nelts = 1 then S.index vs 0
-  else 
-    let lrt = merkle_root_of_pow2 #(nelts / 2) (S.slice vs 0 (nelts / 2)) in
-    let rrt = merkle_root_of_pow2 #(nelts / 2) (S.slice vs (nelts / 2) nelts) in
+  hs:hash_seq_pow2 -> GTot hash (decreases (S.length hs))
+let rec merkle_root_of_pow2 hs =
+  if S.length hs = 1 then S.index hs 0
+  else
+    let lhs, rhs = S.split hs (S.length hs / 2) in
+    let lrt = merkle_root_of_pow2 lhs in
+    let rrt = merkle_root_of_pow2 rhs in
     hash_from_hashes lrt rrt
+
+val merkle_root_of_pow2_inv:
+  hs1:hash_seq_pow2{S.length hs1 > 0} -> 
+  hs2:hash_seq_pow2{S.length hs2 = S.length hs1} ->
+  Lemma (merkle_root_of_pow2 (S.append hs1 hs2) =
+	hash_from_hashes (merkle_root_of_pow2 hs1)
+			 (merkle_root_of_pow2 hs2))
+	[SMTPat (merkle_root_of_pow2 (S.append hs1 hs2))]
+let merkle_root_of_pow2_inv hs1 hs2 =
+  assert (S.length (S.append hs1 hs2) / 2 = S.length hs1);
+  lemma_split_append hs1 hs2
 
 val num_iroots_of: nelts:nat -> GTot nat
 let rec num_iroots_of nelts =
@@ -122,76 +172,144 @@ let rec num_iroots_of nelts =
   else 1 + num_iroots_of (nelts - pow2 (pow2_floor nelts))
 
 val iroots_of_hashes:
-  nelts:nat -> hs:hash_seq{S.length hs = nelts} ->
-  GTot (iroots:hash_seq{S.length iroots = num_iroots_of nelts})
-let rec iroots_of_hashes nelts hs =
-  if nelts = 0 then hs
+  hs:hash_seq -> 
+  GTot (iroots:hash_seq{S.length iroots = num_iroots_of (S.length hs)})
+       (decreases (S.length hs))
+let rec iroots_of_hashes hs =
+  if S.length hs = 0 then hs
   else
-    let n_floor = pow2 (pow2_floor nelts) in
+    let n_floor = pow2 (pow2_floor (S.length hs)) in
     let hs0, hs1 = S.split hs n_floor in
-    S.cons (merkle_root_of_pow2 #n_floor hs0) 
-	   (iroots_of_hashes (nelts - n_floor) hs1)
+    S.cons (merkle_root_of_pow2 hs0) (iroots_of_hashes hs1)
 
-unfold val iroots_of: 
-  nelts:nat -> es:elem_seq{S.length es = nelts} -> GTot hash_seq
-unfold let iroots_of nelts vs =
-  iroots_of_hashes nelts (seq_map hash_from_elem vs)
+val iroots_of_hashes_pow2_same:
+  hs1:hash_seq_pow2 ->
+  hs2:hash_seq{S.length hs2 = S.length hs1} ->
+  Lemma (iroots_of_hashes (S.append hs1 hs2) =
+	S.create 1 (hash_from_hashes 
+	  (S.index (iroots_of_hashes hs1) 0)
+	  (S.index (iroots_of_hashes hs2) 0)))
+
+let iroots_of_hashes_pow2_same hs1 hs2 =
+  S.lemma_eq_elim (S.cons (merkle_root_of_pow2 (S.append hs1 hs2)) S.empty)
+  		  (S.create 1 (merkle_root_of_pow2 (S.append hs1 hs2)));
+  assert (S.index (iroots_of_hashes hs1) 0 = merkle_root_of_pow2 hs1);
+  assert (S.index (iroots_of_hashes hs2) 0 = merkle_root_of_pow2 hs2)
+
+val iroots_of_hashes_pow2_diff:
+  hs1:hash_seq_pow2 ->
+  hs2:hash_seq{S.length hs1 > S.length hs2} ->
+  Lemma (iroots_of_hashes (S.append hs1 hs2) =
+	S.append (iroots_of_hashes hs1) (iroots_of_hashes hs2))
+let iroots_of_hashes_pow2_diff hs1 hs2 =
+  pow2_floor_pow2_less (pow2_floor (S.length hs1)) (S.length hs2);
+  lemma_split_append hs1 hs2;
+  S.lemma_eq_elim
+    (S.cons (merkle_root_of_pow2 hs1) (iroots_of_hashes hs2))
+    (S.append (S.cons (merkle_root_of_pow2 hs1) S.empty)
+	      (iroots_of_hashes hs2))
+
+val iroots_of: elem_seq -> GTot hash_seq
+let iroots_of vs = 
+  iroots_of_hashes (seq_map hash_from_elem vs)
+
+val iroots_of_pow2_same:
+  vs1:elem_seq_pow2 ->
+  vs2:elem_seq{S.length vs2 = S.length vs1} ->
+  Lemma (iroots_of (S.append vs1 vs2) =
+	S.create 1 (hash_from_hashes 
+	  (S.index (iroots_of vs1) 0)
+	  (S.index (iroots_of vs2) 0)))
+let iroots_of_pow2_same vs1 vs2 =
+  seq_map_append hash_from_elem vs1 vs2;
+  iroots_of_hashes_pow2_same
+    (seq_map hash_from_elem vs1)
+    (seq_map hash_from_elem vs2)
+
+val iroots_of_pow2_diff:
+  vs1:elem_seq_pow2 ->
+  vs2:elem_seq{S.length vs1 > S.length vs2} ->
+  Lemma (iroots_of (S.append vs1 vs2) =
+	S.append (iroots_of vs1) (iroots_of vs2))
+let iroots_of_pow2_diff vs1 vs2 =
+  seq_map_append hash_from_elem vs1 vs2;
+  iroots_of_hashes_pow2_diff
+    (seq_map hash_from_elem vs1)
+    (seq_map hash_from_elem vs2)
 
 /// High-level Merkle tree data structure
 
 noeq type merkle_tree =
-| MT: nelts:nat{nelts > 0} -> 
-      values:elem_seq{S.length values = nelts} ->
-      iroots:hash_seq{iroots = iroots_of nelts values} ->
+| MT: values:elem_seq{S.length values > 0} ->
+      iroots:hash_seq{iroots = iroots_of values} ->
       merkle_tree
 
 /// Creating a merkle tree instance
 
 val create_merkle_tree: unit -> merkle_tree
 let create_merkle_tree _ = 
-  S.lemma_eq_elim (iroots_of 1 (S.create 1 elem_init))
+  S.lemma_eq_elim (iroots_of (S.create 1 elem_init))
   		  (S.create 1 (hash_from_elem elem_init));
-  MT 1 (S.create 1 elem_init) (S.create 1 (hash_from_elem elem_init))
+  MT (S.create 1 elem_init) (S.create 1 (hash_from_elem elem_init))
 
 /// Insertion
-
-unfold val insert_nelts: nat -> GTot nat
-unfold let insert_nelts nelts = nelts + 1
 
 val insert_values: elem_seq -> elem -> GTot elem_seq
 let insert_values vs nv = S.snoc vs nv
 
-// val merge_iroots_seq:
-//   sz1:nat -> nelts1:nat{nelts1 = pow2 sz1 && nelts1 < pow2 max_nelts_sz - 1} ->
-//   irs1:hash_seq{S.length irs1 = num_iroots_of max_nelts_sz nelts1} ->
-//   sz2:nat{sz1 >= sz2} -> nelts2:nat{nelts2 = pow2 sz2 && nelts1 + nelts2 < pow2 max_nelts_sz - 1} ->
-//   irs2:hash_seq{S.length irs2 = num_iroots_of max_nelts_sz nelts2} ->
-//   GTot (mirs:hash_seq{S.length mirs = num_iroots_of max_nelts_sz (nelts1 + nelts2)})
-// let merge_iroots_seq sz1 nelts1 irs1 sz2 nelts2 irs2 =
-//   if sz1 = sz2 
-//   then S.create 1 (hash_from_hashes (S.index irs1 0) (S.index irs2 0))
-//   else (pow2_floor_pow2_pow2 sz1 sz2;
-//        assert (num_iroots_of max_nelts_sz nelts1 = 1);
-//        assert (num_iroots_of max_nelts_sz nelts2 = 1);
-//        assert (num_iroots_of max_nelts_sz (nelts1 + nelts2) =
-//        	      1 + num_iroots_of (max_nelts_sz - 1) (nelts1 + nelts2 - pow2 (pow2_floor (nelts1 + nelts2))));
-//        assert (num_iroots_of max_nelts_sz (nelts1 + nelts2) = 2);
-//        S.append irs1 irs2)
+val merge_iroots:
+  vs1:elem_seq_pow2 -> 
+  irs1:hash_seq{iroots_of vs1 = irs1} ->
+  vs2:elem_seq{S.length vs1 >= S.length vs2} ->
+  irs2:hash_seq{iroots_of vs2 = irs2} ->
+  GTot (mirs:hash_seq{iroots_of (S.append vs1 vs2) = mirs})
+let merge_iroots vs1 irs1 vs2 irs2 =
+  if S.length vs1 = S.length vs2
+  then (iroots_of_pow2_same vs1 vs2; 
+       S.create 1 (hash_from_hashes (S.index irs1 0) (S.index irs2 0)))
+  else (iroots_of_pow2_diff vs1 vs2; 
+       S.append irs1 irs2)
 
-val insert_iroots:
-  nelts:nat{nelts > 0} ->
-  irs:hash_seq{S.length irs = num_iroots_of nelts} ->
-  nh:hash ->
-  GTot (iirs:hash_seq{S.length iirs = num_iroots_of (insert_nelts nelts)})
-let rec insert_iroots nelts irs nh =
+val iroots_of_head:
+  vs:elem_seq{S.length vs > 0} ->
+  Lemma (iroots_of (S.slice vs 0 (pow2 (pow2_floor (S.length vs)))) =
+	S.create 1 (S.head (iroots_of vs)))
+let iroots_of_head vs =
   admit ()
 
+val iroots_of_tail:
+  vs:elem_seq{S.length vs > 0} ->
+  Lemma (iroots_of (S.slice vs (pow2 (pow2_floor (S.length vs))) (S.length vs)) =
+	S.tail (iroots_of vs))
+let iroots_of_tail vs =
+  admit ()
+
+val insert_iroots:
+  vs:elem_seq{S.length vs > 0} ->
+  irs:hash_seq{iroots_of vs = irs} ->
+  nv:elem ->
+  GTot (iirs:hash_seq{iroots_of (insert_values vs nv) = iirs})
+       (decreases (S.length irs))
+let rec insert_iroots vs irs nv =
+  if S.length vs = 0
+  then (S.create 1 (hash_from_elem nv))
+  else if is_pow2 (S.length vs)
+  then merge_iroots vs irs (S.create 1 nv) (S.create 1 (hash_from_elem nv))
+  else
+    (let vs0, vs1 = S.split vs (pow2 (pow2_floor (S.length vs))) in
+    lemma_split vs (pow2 (pow2_floor (S.length vs)));
+    iroots_of_head vs;
+    iroots_of_tail vs;
+    append_assoc vs0 vs1 (S.create 1 nv);
+    merge_iroots vs0 (S.create 1 (S.head irs)) (insert_values vs1 nv) 
+		 (insert_iroots vs1 (S.tail irs) nv))
+
+// TODO: refinements
 val insert: mt:merkle_tree -> e:elem -> GTot merkle_tree
 let insert mt e =
-  let nnelts = insert_nelts (MT?.nelts mt) in
-  let niroots = insert_iroots (MT?.nelts mt) (MT?.iroots mt) (hash_from_elem e) in
   let nvalues = insert_values (MT?.values mt) e in
-  admit () // MT nnelts nvalues niroots
+  let niroots = insert_iroots (MT?.values mt) (MT?.iroots mt) e in
+  MT nvalues niroots
 
 /// Getting the Merkle root
 
@@ -216,8 +334,7 @@ let pad_hashes_pow2 vs =
 
 val merkle_root_of_hashes: vs:hash_seq{S.length vs > 0} -> GTot hash
 let merkle_root_of_hashes vs =
-  merkle_root_of_pow2 #(pow2 (padding_to_pow2 (S.length vs))) 
-		      (pad_hashes_pow2 vs)
+  merkle_root_of_pow2 (pad_hashes_pow2 vs)
 
 val merkle_root_of_iroots':
   acc:hash -> irs:hash_seq -> GTot hash (decreases (S.length irs))
